Refactor state

theories/Logic/iFreeSim.v
@@ -1,40 +1,55 @@
 From RSL Require Import Prelude.
 
-From RSL Require Import Commons.Fixpoints.
+From RSL.Commons Require Export WfRel Language.
+From RSL.Logic Require Import Fixpoints.
+
+From iris.proofmode Require Export proofmode.
+
+Class SimInv (PROP : bi) (Λₜ Λₛ : lang) :=
+  {
+    sim_inv : state Λₜ -> state Λₛ -> PROP;
+  }.
 
 Section FSimDef.
+  Context {PROP : bi} `{!BiBUpd PROP, !BiAffine PROP}.
   Context {Λₜ Λₛ: lang}.
   Context (J I: WfRel).
-  Context (Pₜ: prog Λₜ) (Pₛ: prog Λₛ) (S: state Λₜ -> state Λₛ -> rlogic).
+  Context (Pₜ: prog Λₜ) (Pₛ: prog Λₛ).
+  Context {sinv: SimInv PROP Λₜ Λₛ}.
 
-  Abbreviation post := (value Λₜ -> value Λₛ -> rlogic).
-  Abbreviation sim_rel := (post -> state Λₜ -> J -> I -> state Λₛ -> rlogic).
+  Set Default Proof Using "Type*".
 
-  Definition both_final (ϕ: post) (t: state Λₜ) (s: state Λₛ) : rlogic :=
-    ∃ vₜ vₛ, ⌜is_final t = Some vₜ⌟ ∗ ⌜is_final s = Some vₛ⌟ ∗ ϕ vₜ vₛ.
+  Abbreviation post := (value Λₜ -> value Λₛ -> PROP).
+  Abbreviation sim_rel := (post -> state Λₜ -> J -> I -> state Λₛ -> PROP).
+
+  Definition both_final (ϕ: post) (t: state Λₜ) (s: state Λₛ) : PROP :=
+    ∃ vt vs mt ms,
+      ⌜is_final t = Some (vt, mt)⌝ ∗
+      ⌜is_final s = Some (vs, ms)⌝ ∗
+      ϕ vt vs.
 
   Local Definition fsim_body (gfp: sim_rel) (lfp: sim_rel) : sim_rel :=
     fun ϕ t j i s =>
-    ((                          (* Related *)
-      S t s -∗ both_final ϕ t s
-    ) ∨ (                       (* Source Stuck *)
-      ⌜stuck Pₛ s⌝
-    ) ∨ (                       (* Source Steps *)
-      S t s -∗
-      ∃ s' i',
-        ⌜Pₛ ⊨ s ->> s'⌟ ∗ S t s' ∗ lfp ϕ t j i' s'
-    ) ∨ (                       (* Target Steps *)
-      ⌜can_progress Pₜ t⌟ ∗
-      (∀ t',
-         ⌜Pₜ ⊨ t ->> t'⌟ -∗
-         S t s -∗
-         S t' s ∗ ∃ j', lfp ϕ t' j' i s)
-    ) ∨ (                       (* Progress *)
-      ∃ j' i',
-        ⌜j' ⊏ j⌟ ∗
-        ⌜i' ⊏ i⌟ ∗
-        gfp ϕ t j' i' s
-    ))%I.
+      (sim_inv t s ==∗
+       (                          (* Related *)
+         both_final ϕ t s
+       ) ∨ (                       (* Source Stuck *)
+         ⌜stuck Pₛ s⌝
+       ) ∨ (                       (* Source Steps *)
+         ∃ s' i',
+           ⌜Pₛ ⊨ s ->> s'⌝ ∗ sim_inv t s' ∗ lfp ϕ t j i' s'
+       ) ∨ (                       (* Target Steps *)
+         ⌜can_progress Pₜ t⌝ ∗
+         (∀ t',
+            ⌜Pₜ ⊨ t ->> t'⌝ ==∗
+            sim_inv t' s ∗ ∃ j', lfp ϕ t' j' i s)
+       ) ∨ (                       (* Progress *)
+         ∃ j' i',
+           ⌜j' ⊏ j⌝ ∗
+           ⌜i' ⊏ i⌝ ∗
+           gfp ϕ t j' i' s
+       )
+      )%I.
 
   Local Lemma fsim_body_mono gfp1 gfp2 lfp1 lfp2:
     ⊢ □ (∀ ϕ t j i s, gfp1 ϕ t j i s -∗ gfp2 ϕ t j i s) →
@@ -42,21 +57,20 @@ Section FSimDef.
       ∀ ϕ t j i s,
         fsim_body gfp1 lfp1 ϕ t j i s -∗
         fsim_body gfp2 lfp2 ϕ t j i s.
-  Proof using Type.
-    iIntros "#Hgfp #Hlfp" (ϕ t j i s) "Hsim".
-    unfold fsim_body.
+  Proof.
+    iIntros "#Hgfp #Hlfp" (ϕ t j i s) "Hsim Hin".
+    iMod ("Hsim" with "Hin") as "Hsim".
     iDestruct ("Hsim")
       as "[Hfin | [Hstuck | [Hs | [(Hprog & Ht) | Hprog]]]]".
     - do 0 iRight. now iLeft.
     - do 1 iRight. now iLeft.
     - do 2 iRight. iLeft.
-      iIntros "H".
-      iDestruct ("Hs" with "H") as (s' i') "(Hstep & Hstate & Hsim)".
+      iDestruct ("Hs") as (s' i') "(Hstep & Hstate & Hsim)".
       iExists s', i'. iFrame.
       iApply ("Hlfp" with "Hsim").
     - do 3 iRight. iLeft. iFrame.
-      iIntros "%t' H Hstep".
-      iDestruct ("Ht" $! t' with "H Hstep") as "(Hstate & [%j' Hsim])".
+      iModIntro. iIntros "%t' Hstep".
+      iMod ("Ht" with "Hstep") as "(Hstate & [%j' Hsim])".
       iFrame. iExists j'.
       iApply ("Hlfp" with "Hsim").
     - do 4 iRight.
@@ -68,37 +82,36 @@ Section FSimDef.
   Local Lemma fsim_body_mono_strong gfp1 gfp2 lfp1 lfp2:
     ⊢ □ (∀ ϕ ϕ' t j j' i i' s,
            □ (∀ vt vs, ϕ vt vs -∗ ϕ' vt vs) -∗
-           ⌜j ⊑ j'⌟ -∗
-           ⌜i ⊑ i'⌟ -∗
+           ⌜j ⊑ j'⌝ -∗
+           ⌜i ⊑ i'⌝ -∗
            gfp1 ϕ t j i s -∗ gfp2 ϕ' t j' i' s) -∗
       □ (∀ ϕ ϕ' t j j' i i' s,
            □ (∀ vt vs, ϕ vt vs -∗ ϕ' vt vs) -∗
-           ⌜j ⊑ j'⌟ -∗
-           ⌜i ⊑ i'⌟ -∗
+           ⌜j ⊑ j'⌝ -∗
+           ⌜i ⊑ i'⌝ -∗
            lfp1 ϕ t j i s -∗ lfp2 ϕ' t j' i' s) -∗
       ∀ ϕ ϕ' t j j' i i' s,
       □ (∀ vt vs, ϕ vt vs -∗ ϕ' vt vs) -∗
-      ⌜j ⊑ j'⌟ -∗
-      ⌜i ⊑ i'⌟ -∗
+      ⌜j ⊑ j'⌝ -∗
+      ⌜i ⊑ i'⌝ -∗
       fsim_body gfp1 lfp1 ϕ t j i s -∗
       fsim_body gfp2 lfp2 ϕ' t j' i' s.
-  Proof using Type.
-    iIntros "#Hgfp #Hlfp" (ϕ ϕ' t j j' i i' s) "#Hpost %Hj %Hi Hsim".
-    unfold fsim_body.
+  Proof.
+    iIntros "#Hgfp #Hlfp" (ϕ ϕ' t j j' i i' s) "#Hpost %Hj %Hi Hsim Hin".
+    iMod ("Hsim" with "Hin") as "Hsim".
     iDestruct ("Hsim") as "[Hfin | [Hstuck | [Hs | [(Hprog & Ht) | Hprog]]]]".
-    - do 0 iRight. iLeft. iIntros "H".
-      iDestruct ("Hfin" with "H") as "(%vt & %vs & Ht & Hs & Hfin)".
-      iExists vt, vs. iFrame.
+    - do 0 iRight. iLeft.
+      iDestruct ("Hfin") as "(%vt & %vs & %mt & %ms & Ht & Hs & Hfin)".
+      iExists vt, vs, mt, ms. iFrame.
       by iApply ("Hpost" with "Hfin").
     - do 1 iRight. now iLeft.
     - do 2 iRight. iLeft.
-      iIntros "H".
-      iDestruct ("Hs" with "H") as (s' i'') "(Hstep & Hstate & Hsim)".
+      iDestruct ("Hs") as (s' i'') "(Hstep & Hstate & Hsim)".
       iFrame. iExists i''.
       iApply ("Hlfp" with "Hpost [] [] Hsim"); by iPureIntro.
-    - do 3 iRight. iLeft. iFrame.
-      iIntros "%t' H Hstep".
-      iDestruct ("Ht" $! t' with "H Hstep") as "(Hstate & [%j'' Hsim])".
+    - do 3 iRight. iLeft. iFrame. iModIntro.
+      iIntros "%t' Hstep".
+      iMod ("Ht" with "Hstep") as "(Hstate & [%j'' Hsim])".
       iFrame. iExists j''.
       iApply ("Hlfp" with "Hpost [] [] Hsim"); by iPureIntro.
     - do 4 iRight.
@@ -111,7 +124,7 @@ Section FSimDef.
 
   Local Instance fsim_body_bimono gfp :
     BiMonoPred (λ lfp, uncurry5 (fsim_body gfp (curry5 lfp))).
-  Proof using Type.
+  Proof.
     constructor.
     intros lfp1 lfp2. iIntros "#H" (x).
     destruct x as ((((ϕ & t) & j) & i) & s); simpl.
@@ -126,14 +139,14 @@ Section FSimDef.
     curry5 (bi_least_fixpoint (fun lfp => uncurry5 (fsim_body gfp (curry5 lfp)))).
 
   Local Definition fsim_lfp_aux : seal fsim_lfp_def.
-  Proof using Type. by eexists. Qed.
+  Proof. by eexists. Qed.
   Definition fsim_lfp := unseal fsim_lfp_aux.
   Local Lemma fsim_lfp_eq : fsim_lfp = fsim_lfp_def.
-  Proof using Type. exact: seal_eq. Qed.
+  Proof. exact: seal_eq. Qed.
 
   Local Lemma fsim_lfp_unfold gfp ϕ t j i s :
-    fsim_lfp gfp ϕ t j i s ⊣⊢ fsim_body gfp (fsim_lfp gfp) ϕ t j i s.
-  Proof using Type.
+    fsim_lfp gfp ϕ t j i s ≡ fsim_body gfp (fsim_lfp gfp) ϕ t j i s.
+  Proof.
     rewrite fsim_lfp_eq.
     unfold fsim_lfp_def at 1.
     unfold curry5 at 1.
@@ -143,17 +156,18 @@ Section FSimDef.
   Qed.
 
   Lemma fsim_related G ϕ t j i s :
-    ∀ vₜ vₛ,
-    is_final t = Some vₜ ->
-    is_final s = Some vₛ ->
-    ⊢ (S t s -∗ ϕ vₜ vₛ) -∗
+    ∀ vt vs mt ms,
+    is_final t = Some (vt, mt) ->
+    is_final s = Some (vs, ms) ->
+    ⊢ (sim_inv t s ==∗ ϕ vt vs) -∗
       fsim_lfp G ϕ t j i s.
-  Proof using Type.
-    iIntros (vₜ vₛ Ht Hs) "HΦ".
+  Proof.
+    iIntros (vt vs mt ms Ht Hs) "HΦ".
     rewrite fsim_lfp_unfold.
+    iIntros "Hin".
     do 0 iRight. iLeft.
-    iIntros "H". iSpecialize ("HΦ" with "H").
-    iExists vₜ, vₛ.
+    iSpecialize ("HΦ" with "Hin").
+    iExists vt, vs, mt, ms.
     iSplitR. 1: by iPureIntro.
     iSplitR. 1: by iPureIntro.
     now iAssumption.
@@ -162,56 +176,64 @@ Section FSimDef.
   Lemma fsim_source_stuck G ϕ t j i s :
     ⊢ ⌜stuck Pₛ s⌝ -∗
       fsim_lfp G ϕ t j i s.
-  Proof using Type.
+  Proof.
     iIntros "H".
     rewrite fsim_lfp_unfold.
+    iIntros "Hin".
     do 1 iRight. now iLeft.
   Qed.
 
   Lemma fsim_source_steps G ϕ t j i s :
-    ⊢ (S t s -∗
-       ∃ s' i', ⌜Pₛ ⊨ s ->> s'⌟ ∗ S t s' ∗ fsim_lfp G ϕ t j i' s') -∗
+    ⊢ (sim_inv t s ==∗
+       ∃ s' i', ⌜Pₛ ⊨ s ->> s'⌝ ∗ sim_inv t s' ∗ fsim_lfp G ϕ t j i' s') -∗
     fsim_lfp G ϕ t j i s.
-  Proof using Type.
+  Proof.
     iIntros "Hs".
     rewrite fsim_lfp_unfold.
-    do 2 iRight. now iLeft.
+    iIntros "Hin".
+    do 2 iRight. iLeft.
+    now iApply ("Hs" with "Hin").
   Qed.
 
   Lemma fsim_target_steps G ϕ t j i s :
     can_progress Pₜ t ->
     ⊢ (∀ t',
-       ⌜Pₜ ⊨ t ->> t'⌟ -∗
-       S t s -∗
-       S t' s ∗ ∃ j', fsim_lfp G ϕ t' j' i s) -∗
+         ⌜Pₜ ⊨ t ->> t'⌝ -∗
+         sim_inv t s ==∗
+         sim_inv t' s ∗ ∃ j', fsim_lfp G ϕ t' j' i s) -∗
       fsim_lfp G ϕ t j i s.
-  Proof using Type.
+  Proof.
     iIntros (H) "Ht".
     rewrite fsim_lfp_unfold.
+    iIntros "Hin".
     do 3 iRight. iLeft.
     iSplitR.
     - by iPureIntro.
-    - by iAssumption.
+    - iModIntro. iIntros (t' Hstep).
+      by iApply ("Ht" with "[//] Hin").
   Qed.
 
   Lemma fsim_progress G ϕ t j i s:
     ∀ j' i',
     j' ⊏ j ->
     i' ⊏ i ->
-    ⊢ G ϕ t j' i' s -∗ fsim_lfp G ϕ t j i s.
-  Proof using Type.
+    ⊢ (sim_inv t s ==∗ G ϕ t j' i' s) -∗
+      fsim_lfp G ϕ t j i s.
+  Proof.
     iIntros (j' i' Hj Hi) "Hf".
     rewrite fsim_lfp_unfold.
+    iIntros "Hin".
+    iMod ("Hf" with "Hin") as "Hf".
     do 4 iRight.
-    iExists j', i'. iFrame. by iSplit.
+    iExists j', i'. iFrame. by iPureIntro.
   Qed.
 
-  Local Lemma fsim_lfp_strong_ind (P R: sim_rel):
+  Lemma fsim_lfp_ind (P R: sim_rel):
     ⊢ (□ ∀ ϕ t j i s,
          fsim_body R (fun ϕ t j i s => P ϕ t j i s ∧ fsim_lfp R ϕ t j i s) ϕ t j i s -∗
          P ϕ t j i s) -∗
     ∀ ϕ t j i s, fsim_lfp R ϕ t j i s -∗ P ϕ t j i s.
-  Proof using Type.
+  Proof.
     iIntros "#IH" (ϕ t j i s) "H".
     rewrite fsim_lfp_eq.
     unfold fsim_lfp. unfold curry5.
@@ -222,55 +244,13 @@ Section FSimDef.
     iApply ("IH" with "H").
   Qed.
 
-  Lemma fsim_lfp_ind (P R: sim_rel):
-    ⊢ (* Related *)
-      (□ ∀ ϕ t j i s,
-        (S t s -∗ both_final ϕ t s) -∗ P ϕ t j i s) -∗
-      (* Source Stuck *)
-      (□ ∀ ϕ t j i s,
-        ⌜stuck Pₛ s⌝ -∗ P ϕ t j i s) -∗
-      (* Source Steps *)
-      (□ ∀ ϕ t j i s,
-         (S t s -∗
-          ∃ s' i',
-            ⌜Pₛ ⊨ s ->> s'⌟ ∗
-            S t s' ∗
-            P ϕ t j i' s' ∧ fsim_lfp R ϕ t j i' s') -∗
-         P ϕ t j i s) -∗
-      (* Target Steps *)
-      (□ ∀ ϕ t j i s,
-        (⌜can_progress Pₜ t⌟ ∗
-         (∀ t',
-            ⌜Pₜ ⊨ t ->> t'⌟ -∗
-            S t s -∗
-            S t' s ∗ ∃ j', P ϕ t' j' i s ∧ fsim_lfp R ϕ t' j' i s)
-        ) -∗
-        P ϕ t j i s) -∗
-      (* Progress *)
-      (□ ∀ ϕ t j j' i i' s,
-        ⌜j' ⊏ j⌟ -∗ ⌜i' ⊏ i⌟ -∗ R ϕ t j' i' s -∗ P ϕ t j i s) -∗
-      (* Conclusion *)
-      ∀ ϕ t j i s, fsim_lfp R ϕ t j i s -∗ P ϕ t j i s.
-  Proof using Type.
-    iIntros "#IHfin #IHstuck #IHsstep #IHtstep #IHprog" (ϕ t j i s) "H".
-    iApply (fsim_lfp_strong_ind with "[] H").
-    clear ϕ t j i s. iIntros "!>" (ϕ t j i s) "H".
-    iDestruct ("H") as "[Hfin | [Hstuck | [Hs | [(H & Ht) | H]]]]".
-    - by iApply ("IHfin" with "Hfin").
-    - by iApply ("IHstuck" with "Hstuck").
-    - by iApply ("IHsstep").
-    - iApply ("IHtstep"). by iFrame.
-    - iDestruct "H" as (j' i') "(Hj & Hi & HR)".
-      by iApply ("IHprog" with "Hj Hi HR").
-  Qed.
-
   Lemma fsim_lfp_mono gfp gfp' ϕ t j i s :
     ⊢ □ (∀ ϕ t j i s, gfp ϕ t j i s -∗ gfp' ϕ t j i s) -∗
       fsim_lfp gfp ϕ t j i s -∗
       fsim_lfp gfp' ϕ t j i s.
-  Proof using Type.
+  Proof.
     iIntros "#Hgfp Hsim".
-    iApply (fsim_lfp_strong_ind with "[] Hsim"); clear.
+    iApply (fsim_lfp_ind with "[] Hsim"); clear.
     iIntros "!>" (ϕ t j i s) "IH".
     rewrite fsim_lfp_unfold.
     iApply (fsim_body_mono with "Hgfp [] IH").
@@ -278,30 +258,30 @@ Section FSimDef.
     by iApply bi.and_elim_l.
   Qed.
 
-  Local Definition fsim_lfp_mono_inv R ϕ t j i s : rlogic :=
+  Local Definition fsim_lfp_mono_inv R ϕ t j i s : PROP :=
     ∀ ϕ' j' i',
     □ (∀ vt vs, ϕ vt vs -∗ ϕ' vt vs) -∗
-    ⌜j ⊑ j'⌟ -∗
-    ⌜i ⊑ i'⌟ -∗
+    ⌜j ⊑ j'⌝ -∗
+    ⌜i ⊑ i'⌝ -∗
     fsim_lfp R ϕ' t j' i' s.
 
   Lemma fsim_lfp_mono_strong gfp gfp' ϕ ϕ' t j j' i i' s :
     ⊢ □ (∀ ϕ ϕ' t j j' i i' s,
            □ (∀ vt vs, ϕ vt vs -∗ ϕ' vt vs) -∗
-           ⌜j ⊑ j'⌟ -∗
-           ⌜i ⊑ i'⌟ -∗
+           ⌜j ⊑ j'⌝ -∗
+           ⌜i ⊑ i'⌝ -∗
            gfp ϕ t j i s -∗
            gfp' ϕ' t j' i' s) -∗
       □ (∀ vt vs, ϕ vt vs -∗ ϕ' vt vs) -∗
-      ⌜j ⊑ j'⌟ -∗
-      ⌜i ⊑ i'⌟ -∗
+      ⌜j ⊑ j'⌝ -∗
+      ⌜i ⊑ i'⌝ -∗
       fsim_lfp gfp ϕ t j i s -∗
       fsim_lfp gfp' ϕ' t j' i' s.
-  Proof using Type.
+  Proof.
     iIntros "#Hgfp Hpost Hj Hi Hsim".
     iAssert (fsim_lfp_mono_inv gfp' ϕ t j i s) with "[Hsim]" as "H".
     {
-      iApply (fsim_lfp_strong_ind (fsim_lfp_mono_inv gfp') with "[] Hsim").
+      iApply (fsim_lfp_ind (fsim_lfp_mono_inv gfp') with "[] Hsim").
       clear.
       iIntros "!>" (ϕ t j i s) "IH".
       iIntros (ϕ' j' i') "Hpost Hj Hi".
@@ -317,7 +297,7 @@ Section FSimDef.
 
   Local Instance fsim_gfp_def_mono :
     BiMonoPred (fun gfp => uncurry5 (fsim_lfp (curry5 gfp))).
-  Proof using Type.
+  Proof.
     constructor.
     intros gfp1 gfp2. iIntros "#Hgfp" (x).
     destruct x as ((((ϕ & t) & j) & i) & s); simpl.
@@ -333,7 +313,7 @@ Section FSimDef.
 
   Local Lemma fsim_gfp_def_unfold ϕ t j i s :
     fsim_gfp_def ϕ t j i s ≡ fsim_lfp fsim_gfp_def ϕ t j i s.
-  Proof using Type.
+  Proof.
     unfold fsim_gfp_def at 1.
     unfold curry5 at 1.
     rewrite greatest_fixpoint_unfold.
@@ -343,7 +323,7 @@ Section FSimDef.
 
   Local Lemma fsim_gfp_def_fixpoint ϕ t j i s:
     fsim_gfp_def ϕ t j i s ≡ fsim_body fsim_gfp_def fsim_gfp_def ϕ t j i s.
-  Proof using Type.
+  Proof.
     rewrite fsim_gfp_def_unfold fsim_lfp_unfold.
     iSplit.
     - iIntros "H". iApply (fsim_body_mono with "[] [] H"); auto.
@@ -357,14 +337,14 @@ Section FSimDef.
   (** * Free Simulation *)
 
   Local Definition fsim_aux : seal fsim_gfp_def.
-  Proof using Type. by eexists. Qed.
+  Proof. by eexists. Qed.
   Definition fsim := unseal fsim_aux.
   Local Lemma fsim_eq : fsim = fsim_gfp_def.
-  Proof using Type. unfold fsim. by rewrite (seal_eq fsim_aux). Qed.
+  Proof. unfold fsim. by rewrite (seal_eq fsim_aux). Qed.
 
   Lemma fsim_fixpoint ϕ t j i s:
-    fsim ϕ t j i s ⊣⊢ fsim_lfp fsim ϕ t j i s.
-  Proof using Type. rewrite fsim_eq. by apply fsim_gfp_def_unfold. Qed.
+    fsim ϕ t j i s ≡ fsim_lfp fsim ϕ t j i s.
+  Proof. rewrite fsim_eq. by apply fsim_gfp_def_unfold. Qed.
 
   Lemma fsim_coind_strong (P: sim_rel) :
     ⊢ (□ ∀ ϕ t j i s,
@@ -373,7 +353,7 @@ Section FSimDef.
            (λ ϕ t j i s, P ϕ t j i s ∨ fsim ϕ t j i s) ϕ t j i s
       ) -∗
     ∀ ϕ t j i s, P ϕ t j i s -∗ fsim ϕ t j i s.
-  Proof using Type.
+  Proof.
     iIntros "#CIH" (ϕ t j i s) "HP".
     rewrite fsim_eq. unfold  fsim_gfp_def, curry5.
     set (Pcur := uncurry5 P).
@@ -388,36 +368,37 @@ Section FSimDef.
     ⊢ (□ ∀ R ϕ t j i s,
          (□ ∀ ϕ t j j' i i' s,
             P ϕ t j i s -∗
-            ⌜j ⊏ j'⌟ -∗
-            ⌜i ⊏ i'⌟ -∗
+            ⌜j ⊏ j'⌝ -∗
+            ⌜i ⊏ i'⌝ -∗
             fsim_lfp R ϕ t j' i' s) -∗
          P ϕ t j i s -∗
          fsim_lfp R ϕ t j i s) -∗
     ∀ ϕ t j i s, P ϕ t j i s -∗ fsim ϕ t j i s.
-  Proof using Type.
+  Proof.
     iIntros "#CIH" (ϕ t j i s) "HP".
     iApply (fsim_coind_strong with "[] HP").
     clear. iIntros "!>" (ϕ t j i s) "HP".
     iApply ("CIH" with "[] HP").
     clear. iIntros "!>" (ϕ t j j' i i' s) "HP %Hj %Hi".
     iApply ((fsim_progress _ _ _ _ _ _ _ _ Hj Hi)).
+    iIntros "Hin".
     by iLeft.
   Qed.
 
-  Local Definition fsim_mono_coind_inv ϕ' t j' i' s : rlogic :=
+  Local Definition fsim_mono_coind_inv ϕ' t j' i' s : PROP :=
     ∃ ϕ j i,
       □ (∀ vt vs, ϕ vt vs -∗ ϕ' vt vs) ∗
-      ⌜j ⊑ j'⌟ ∗
-      ⌜i ⊑ i'⌟ ∗
+      ⌜j ⊑ j'⌝ ∗
+      ⌜i ⊑ i'⌝ ∗
       fsim_gfp_def ϕ t j i s.
 
   Lemma fsim_mono ϕ ϕ' t j j' i i' s:
     ⊢ □ (∀ vt vs, ϕ vt vs -∗ ϕ' vt vs) -∗
-      ⌜j ⊑ j'⌟ -∗
-      ⌜i ⊑ i'⌟ -∗
+      ⌜j ⊑ j'⌝ -∗
+      ⌜i ⊑ i'⌝ -∗
       fsim ϕ t j i s -∗
       fsim ϕ' t j' i' s.
-  Proof using Type.
+  Proof.
     iIntros "Hmon Hj Hi Hsim".
     iApply (fsim_coind_strong fsim_mono_coind_inv).
     {
