theories/Commons/Language.v
@@ -1,0 +1,112 @@
+From RSL Require Import Prelude.
+From RSL Require Export Commons.Memory.
+
+Section lang_mixin.
+  Context {prog pstate value : Type}.
+
+  Context (step_rel : prog -> (pstate * memory) -> (pstate * memory) -> Prop).
+  Context (is_final : (pstate * memory) -> option (value * memory)).
+
+  Record LangMixin := {
+      mixin_final_no_step:
+      ∀ s v m,
+        is_final s = Some (v, m) ->
+        ∀ p s', ~step_rel p s s';
+    }.
+End lang_mixin.
+
+Structure lang :=
+  Lang
+    {
+      prog : Type;
+      pstate : Type;
+      value : Type;
+
+      step_rel : prog -> (pstate * memory) -> (pstate * memory) -> Prop;
+      is_final : (pstate * memory) -> option (value * memory);
+
+      lang_mixin : LangMixin step_rel is_final;
+    }.
+
+Arguments step_rel {_} _ _ _.
+Arguments is_final {_} _.
+
+Notation "P ⊨ s '->>' t" := (step_rel P s t) (at level 60, right associativity).
+Notation "P ⊨ s '-{' n '}>' t" := (nsteps (step_rel P) n s t) (at level 60, right associativity).
+Notation "P ⊨ s '->>*' t" := (rtc (step_rel P) s t) (at level 60, right associativity).
+Notation "P ⊨ s '->>+' t" := (psteps (step_rel P) s t) (at level 60, right associativity).
+
+Definition state (Λ: lang) : Type := pstate Λ * memory.
+
+Definition pstate_of_state {Λ : lang} : state Λ -> pstate Λ := fst.
+Definition memory_of_state {Λ : lang} : state Λ -> memory := snd.
+
+Section LangProp.
+  Context {Λ: lang} (P: prog Λ).
+
+  Lemma final_no_step s:
+    is_Some (is_final s) -> ∀ t, ~(P ⊨ s ->> t).
+  Proof using Type.
+    intros [[] Hf] t. eapply mixin_final_no_step.
+    - apply lang_mixin.
+    - exact Hf.
+  Qed.
+
+  Definition can_progress (s: state Λ): Prop :=
+    ∃ t, P ⊨ s ->> t.
+
+  Definition stuck (s: state Λ) : Prop :=
+    is_final s = None ∧ ~ can_progress s.
+
+  Lemma can_progress_must_step s:
+    can_progress s -> ∃ t, P ⊨ s ->> t.
+  Proof using Type. easy. Qed.
+
+  Lemma final_no_progress s:
+    is_Some (is_final s) -> ~can_progress s.
+  Proof using Type.
+    intros [[] Hfin] Hp. destruct (can_progress_must_step _ Hp) as (? & H).
+    eapply mixin_final_no_step.
+    - apply lang_mixin.
+    - eassumption.
+    - exact H.
+  Qed.
+
+  Lemma final_not_stuck s:
+    is_Some (is_final s) -> ~ stuck s.
+  Proof using Type.
+    intros [[] Hfin] [Hnstuck _]. congruence.
+  Qed.
+
+  Lemma progress_not_stuck s:
+    can_progress s -> ~ stuck s.
+  Proof using Type. intros H [_ Hnprog]. by eapply Hnprog. Qed.
+End LangProp.
+
+Section TwoProg.
+  Context {Λₜ Λₛ: lang}.
+  Context (Pₜ : prog Λₜ) (Pₛ : prog Λₛ).
+
+  Abbreviation post := (value Λₜ * memory -> value Λₛ * memory -> Prop).
+
+  Definition both_final (ϕ: post) (t: state Λₜ) (s: state Λₛ) : Prop :=
+    ∃ vt vs,
+      is_final t = Some vt ∧
+      is_final s = Some vs ∧
+      ϕ vt vs.
+
+End TwoProg.
+
+Ltac langmixin :=
+  match goal with
+  | [ Hf: is_final ?s = Some _, Hp: can_progress _ ?s |- _ ] =>
+      exfalso; now apply (final_no_progress _ _ (mk_is_Some _ _ Hf) Hp)
+  | [ Hf: is_final ?s = Some _, Hs: _ ⊨ ?s ->> _ |- _ ] =>
+      exfalso; now apply (final_no_step _ _ (mk_is_Some _ _ Hf) _ Hs)
+  | [ Hf: is_final ?s = Some _, Hs: stuck _ ?s |- _ ] =>
+      exfalso; now apply (final_not_stuck _ _ (mk_is_Some _ _ Hf) Hs)
+  | [ Hs: stuck ?P ?s, Hp: can_progress ?P ?s |- _ ] =>
+      exfalso; now apply (progress_not_stuck _ _ Hp Hs)
+  | [ Hfin: both_final _ _ _ |- _ ] =>
+      destruct Hfin as (? & ? & ? & ? & ?); now langmixin
+  end.
