theories/Logic/MemoryInv.v
@@ -1,0 +1,181 @@
+From RSL Require Import Prelude.
+
+From RSL.Logic Require Import GSetView.
+From RSL.Commons Require Import Language.
+
+From iris.base_logic.lib Require Import own ghost_map.
+From iris.proofmode Require Import proofmode.
+
+Class memGpreS Σ :=
+  MemGpreS {
+      #[local] mem_pre_heapG :: ghost_mapG Σ loc val;
+      #[local] mem_pre_freedG :: gset_viewG Σ loc;
+    }.
+
+Class memGS Σ :=
+  MemGS {
+      #[local] mem_inG :: memGpreS Σ;
+
+      gen_heap_name : gname;
+      gen_freed_name : gname
+    }.
+
+Arguments MemGS Σ {_} _ _.
+Arguments gen_heap_name {Σ} _.
+Arguments gen_freed_name {Σ} _.
+
+Definition memΣ : gFunctors :=
+  #[ ghost_mapΣ loc val; gset_viewΣ loc ].
+
+Global Instance subG_MemΣ {Σ} : subG memΣ Σ → memGpreS Σ.
+Proof. solve_inG. Qed.
+
+Section memory_defs.
+  Context `{HinG : memGS Σ}.
+
+  Local Definition memory_inv_def (m: memory): iProp Σ :=
+    ∃ freed,
+      ghost_map_auth (gen_heap_name HinG) 1%Qp m ∗
+      gset_view_own_auth (gen_freed_name HinG) (DfracOwn 1) freed ∗
+      ⌜∀ l, l ∈ freed -> m !! l = None⌝.
+
+  Local Definition memory_inv_aux : seal (@memory_inv_def).
+  Proof using Type. by eexists. Qed.
+  Definition memory_inv := unseal memory_inv_aux.
+  Local Lemma memory_inv_eq : @memory_inv = @memory_inv_def.
+  Proof using Type. by apply seal_eq. Qed.
+
+  Local Definition pointsto_def (l : loc) (dq : dfrac) (v : val) : iProp Σ :=
+    ghost_map_elem (gen_heap_name HinG) l dq v.
+
+  Local Definition pointsto_aux : seal (@pointsto_def).
+  Proof using Type. by eexists. Qed.
+  Definition pointsto := unseal pointsto_aux.
+  Local Lemma pointsto_eq : @pointsto = @pointsto_def.
+  Proof using Type. by apply seal_eq. Qed.
+
+  Definition freed_def (l : loc) : iProp Σ :=
+    gset_view_own_elem (gen_freed_name HinG) l.
+
+  Local Definition freed_aux : seal (@freed_def).
+  Proof using Type. by eexists. Qed.
+  Definition freed := unseal freed_aux.
+  Local Lemma freed_eq : @freed = @freed_def.
+  Proof using Type. by apply seal_eq. Qed.
+End memory_defs.
+
+Local Ltac unseal :=
+  rewrite
+    ?memory_inv_eq /memory_inv_def
+    ?pointsto_eq /pointsto_def
+    ?freed_eq /freed_def.
+
+Section memory_laws.
+  Context `{!memGS Σ}.
+
+  Local Notation "l ↦ v" :=
+    (pointsto l (DfracOwn 1) v)
+      (at level 20) : bi_scope.
+
+  Local Notation "'free' l" :=
+    (freed l)
+      (at level 20) : bi_scope.
+
+  Lemma mapsto_valid l v: l ↦ v -∗ ⌜✓ DfracOwn 1⌝.
+  Proof using Type. unseal. by iApply ghost_map_elem_valid. Qed.
+
+  Lemma mapsto_valid_2 l v1 v2: l ↦ v1 -∗ l ↦ v2 -∗ False.
+  Proof using Type.
+    unseal. iIntros "H1 H2".
+    iDestruct (ghost_map_elem_valid_2 with "H1 H2") as "[%H _]".
+    exfalso. by apply dfrac_valid_own in H.
+  Qed.
+
+  Lemma pointsto_interp m l v:
+    memory_inv m -∗
+    l ↦ v -∗
+    ⌜m !! l = Some v⌝.
+  Proof using Type.
+    unseal. iIntros "(%f & Hm & Hf & %Hinv) Hl".
+    by iApply (ghost_map_lookup with "Hm Hl").
+  Qed.
+
+  Lemma free_interp m l:
+    memory_inv m -∗
+    free l -∗
+    ⌜m !! l = None⌝.
+  Proof using Type.
+    unseal. iIntros "(%f & Hm & Hf & %Hinv) Hl".
+    iDestruct (gset_view_elem_of with "Hf Hl") as "%".
+    iPureIntro. by apply Hinv.
+  Qed.
+
+  (** Update lemmas *)
+  Lemma memory_alloc m v:
+    memory_inv m ==∗
+    ∃ l, ⌜m !! l = None⌝ ∗
+         memory_inv (<[l := v]>m) ∗ l ↦ v.
+  Proof using Type.
+    unseal.
+    iIntros "(%f & Hm & Hf & %Hinv)".
+    set (l := fresh (dom m ∪ f)).
+    assert (m !! l = None).
+    { apply not_elem_of_dom. intro Hf.
+      eapply elem_of_union_l in Hf. apply (is_fresh _ Hf).
+    }
+    iMod (ghost_map_insert l v with "Hm") as "[Hm Hl]"; first done.
+    iFrame. iPureIntro. split; auto.
+    intros l' Hin. rewrite lookup_insert_ne; auto.
+    intros <-. subst l.
+    eapply elem_of_union_r in Hin.
+    apply (is_fresh _ Hin).
+  Qed.
+
+  Lemma memory_update m l vold v:
+    memory_inv m -∗
+    l ↦ vold ==∗
+    memory_inv (<[l := v]>m) ∗ l ↦ v.
+  Proof using Type.
+    unseal.
+    iIntros "(%f & Hm & Hf & %Hinv) Hl".
+    iDestruct (ghost_map_lookup with "Hm Hl") as "%Hv".
+    iMod (ghost_map_update with "Hm Hl") as "[Hm Hl]".
+    iModIntro. iFrame.
+    iPureIntro. intros l' Hin.
+    rewrite lookup_insert_ne; auto.
+    intros ->. apply Hinv in Hin.
+    by rewrite Hv in Hin.
+  Qed.
+
+  Lemma memory_free m l v:
+    memory_inv m -∗
+    l ↦ v ==∗
+    memory_inv (delete l m) ∗ free l.
+  Proof using Type.
+    unseal.
+    iIntros "(%f & Hm & Hf & %Hinv) Hl".
+    iDestruct (ghost_map_lookup with "Hm Hl") as "%Hv".
+    iMod (ghost_map_delete with "Hm Hl") as "Hm".
+    iMod (gset_view_own_extend l with "Hf") as "[Hf Hfree]".
+    { intros Hin. apply Hinv in Hin. by rewrite Hv in Hin. }
+    iModIntro. iFrame.
+    iPureIntro. intros l' Hin.
+    rewrite elem_of_union elem_of_singleton in Hin.
+    destruct Hin as [-> | Hin].
+    - by apply lookup_delete_eq.
+    - rewrite lookup_delete_ne; auto.
+      intros ->. apply Hinv in Hin. by rewrite Hv in Hin.
+  Qed.
+
+End memory_laws.
+
+Lemma memory_init `{!memGpreS Σ} m :
+  ⊢ |==> ∃ _ : memGS Σ,
+    memory_inv m ∗ ([∗ map] l ↦ v ∈ m, pointsto l (DfracOwn 1) v).
+Proof.
+  iMod (ghost_map_alloc m (K:=loc) (V:=val)) as (heap_name) "[Hm Hl]".
+  iMod (gset_view_own_alloc_empty (A := loc)) as (free_name) "Hf".
+  iExists (MemGS Σ heap_name free_name).
+  unseal. simpl. iFrame.
+  iPureIntro. discriminate.
+Qed.
